src/lang/Thread.v
@@ -20,27 +20,27 @@ Set Implicit Arguments.
 Module Local.
   Structure t := mk {
     commit: Commit.t;
-    promises: Promises.t;
+    promises: Memory.t;
   }.
 
-  Definition init := mk Commit.elt Promises.bot.
+  Definition init := mk Commit.elt Memory.bot.
 
   Inductive is_terminal (lc:t): Prop :=
   | is_terminal_intro
-      (PROMISES: lc.(promises) = Promises.bot)
+      (PROMISES: lc.(promises) = Memory.bot)
   .
 
   Inductive wf (lc:t) (mem:Memory.t): Prop :=
   | wf_intro
       (COMMIT_WF: Commit.wf lc.(commit))
       (COMMIT_CLOSED: Commit.closed lc.(commit) mem)
-      (PROMISES: Memory.closed_promises lc.(promises) mem)
+      (PROMISES: Memory.le lc.(promises) mem)
       (MEMORY: Memory.closed mem)
   .
 
   Inductive disjoint (lc1 lc2:t): Prop :=
   | disjoint_intro
-      (PROMISES: Promises.disjoint lc1.(promises) lc2.(promises))
+      (DISJOINT: Memory.disjoint lc1.(promises) lc2.(promises))
   .
 
   Global Program Instance disjoint_Symmetric: Symmetric disjoint.
@@ -81,7 +81,7 @@ Module Local.
   Inductive fulfill_step (lc1:t) (mem1:Memory.t) (loc:Loc.t) (from to:Time.t) (val:Const.t) (releasedc releasedm:Capability.t) (ord:Ordering.t): forall (lc2:t), Prop :=
   | step_fulfill
       commit2 promises2
-      (FULFILL: Memory.fulfill lc1.(promises) mem1 loc from to (Message.mk val releasedm) promises2)
+      (FULFILL: Memory.fulfill lc1.(promises) loc from to (Message.mk val releasedm) promises2)
       (COMMIT: Commit.write lc1.(commit) loc to releasedc ord commit2)
       (COMMIT_WF: Commit.wf commit2)
       (COMMIT_CLOSED: Commit.closed commit2 mem1):
@@ -92,13 +92,13 @@ Module Local.
   | step_write_fulfill
       lc2
       (FULFILL: fulfill_step lc1 mem1 loc from to val releasedc releasedm ord lc2)
-      (RELEASE: Ordering.le Ordering.acqrel ord -> lc1.(promises) loc = DOSet.empty):
+      (RELEASE: Ordering.le Ordering.acqrel ord -> lc1.(promises) loc = Cell.bot):
       write_step lc1 mem1 loc from to val releasedc releasedm ord lc2 mem1
   | step_write_add
       lc2 mem2 lc3
       (PROMISE: promise_step lc1 mem1 loc from to val releasedm lc2 mem2)
       (FULFILL: fulfill_step lc2 mem2 loc from to val releasedc releasedm ord lc3)
-      (RELEASE: Ordering.le Ordering.acqrel ord -> lc1.(promises) loc = DOSet.empty):
+      (RELEASE: Ordering.le Ordering.acqrel ord -> lc1.(promises) loc = Cell.bot):
       write_step lc1 mem1 loc from to val releasedc releasedm ord lc3 mem2
   .
 
@@ -107,23 +107,11 @@ Module Local.
       commit2 commit3
       (READ: Commit.read_fence lc1.(commit) ordr commit2)
       (WRITE: Commit.write_fence commit2 ordw commit3)
-      (RELEASE: Ordering.le Ordering.acqrel ordw -> lc1.(promises) = Promises.bot)
+      (RELEASE: Ordering.le Ordering.acqrel ordw -> lc1.(promises) = Memory.bot)
       (COMMIT_WF: Commit.wf commit3)
       (COMMIT_CLOSED: Commit.closed commit3 mem1):
       fence_step lc1 mem1 ordr ordw (mk commit3 lc1.(promises))
   .
-
-  Lemma future_wf lc mem1 mem1'
-        (WF: wf lc mem1)
-        (FUTURE: Memory.future mem1 mem1')
-        (INTACT: Memory.intact lc.(promises) mem1 mem1'):
-    wf lc mem1'.
-  Proof.
-    inv WF. econs; eauto.
-    - eapply Commit.future_closed; eauto.
-    - eapply Memory.future_closed_promises; eauto.
-    - eapply Memory.future_closed; eauto.
-  Qed.
 
   Lemma future_read_step lc1 mem1 mem1' loc ts val released ord lc2
         (FUTURE: Memory.future mem1 mem1')
@@ -136,13 +124,11 @@ Module Local.
 
   Lemma future_fulfill_step lc1 mem1 mem1' loc from to val releasedc releasedm ord lc2
         (FUTURE: Memory.future mem1 mem1')
-        (INTACT: Memory.intact lc1.(promises) mem1 mem1')
         (STEP: fulfill_step lc1 mem1 loc from to val releasedc releasedm ord lc2):
     fulfill_step lc1 mem1' loc from to val releasedc releasedm ord lc2.
   Proof.
     inv STEP. econs; eauto.
-    - eapply Memory.fulfill_mon; eauto.
-    - eapply Commit.future_closed; eauto.
+    eapply Commit.future_closed; eauto.
   Qed.
 
   Lemma future_fence_step lc1 mem1 mem1' ordr ordw lc2
@@ -197,7 +183,7 @@ Module Local.
     <<FUTURE: Memory.future mem1 mem2>>.
   Proof.
     inv STEP.
-    - exploit fulfill_step_future; eauto. i. splits; ss. reflexivity.
+    - exploit fulfill_step_future; eauto. i. splits; ss. refl.
     - exploit promise_step_future; eauto. i. des.
       exploit fulfill_step_future; eauto.
   Qed.
@@ -217,13 +203,12 @@ Module Local.
         (DISJOINT1: disjoint lc1 lc)
         (WF: wf lc mem1):
     <<DISJOINT2: disjoint lc2 lc>> /\
-    <<INTACT: Memory.intact lc.(Local.promises) mem1 mem2>> /\
     <<WF: wf lc mem2>>.
   Proof.
     inv WF1. inv DISJOINT1. inversion WF. inv STEP.
     exploit Memory.promise_future; try apply PROMISE; eauto. i. des.
     exploit Memory.promise_disjoint; try apply PROMISE; eauto. i. des.
-    splits; ss. eapply Local.future_wf; eauto.
+    splits; ss. econs; eauto. eapply Commit.future_closed; eauto.
   Qed.
 
   Lemma silent_step_disjoint
@@ -251,12 +236,15 @@ Module Local.
   Lemma fulfill_step_disjoint
         lc1 mem1 lc2 loc from to val releasedc releasedm ord lc
         (STEP: fulfill_step lc1 mem1 loc from to val releasedc releasedm ord lc2)
-        (DISJOINT1: disjoint lc1 lc):
+        (WF1: wf lc1 mem1)
+        (DISJOINT1: disjoint lc1 lc)
+        (WF: wf lc mem1):
     disjoint lc2 lc.
   Proof.
-    inv DISJOINT1. inv STEP. inv FULFILL.
-    econs. s. econs. i. eapply PROMISES; try apply RHS; eauto.
-    apply Promises.unset_inv in LHS. des. auto.
+    inv WF1. inv DISJOINT1. inversion WF. inv STEP.
+    hexploit Memory.fulfill_future; try apply FULFILL; eauto. i. des.
+    hexploit Memory.fulfill_disjoint; try apply FULFILL; try apply DISJOINT; eauto. i. des.
+    econs. auto.
   Qed.
 
   Lemma write_step_disjoint
@@ -266,12 +254,11 @@ Module Local.
         (DISJOINT1: disjoint lc1 lc)
         (WF: wf lc mem1):
     <<DISJOINT2: disjoint lc2 lc>> /\
-    <<INTACT: Memory.intact lc.(Local.promises) mem1 mem2>> /\
     <<WF: wf lc mem2>>.
   Proof.
     inv STEP.
-    - exploit fulfill_step_disjoint; eauto. i.
-      splits; eauto. reflexivity.
+    - exploit fulfill_step_future; eauto. i. des.
+      exploit fulfill_step_disjoint; eauto.
     - exploit promise_step_future; eauto. i. des.
       exploit promise_step_disjoint; eauto. i. des.
       exploit fulfill_step_disjoint; eauto.
@@ -363,10 +350,10 @@ Module Thread.
     Definition consistent st1 lc1 mem: Prop :=
       forall mem1
         (FUTURE: Memory.future mem mem1)
-        (INTACT: Memory.intact lc1.(Local.promises) mem mem1),
+        (WF: Local.wf lc1 mem1),
       exists e2,
         <<STEPS: rtc (step None) (mk st1 lc1 mem1) e2>> /\
-        <<PROMISES: e2.(local).(Local.promises) = Promises.bot>>.
+        <<PROMISES: e2.(local).(Local.promises) = Memory.bot>>.
 
     Lemma promise_step_future e1 e2
           (STEP: promise_step e1 e2)
@@ -384,12 +371,12 @@ Module Thread.
       <<FUTURE: Memory.future e1.(memory) e2.(memory)>>.
     Proof.
       inv STEP; s.
-      - exploit Local.silent_step_future; eauto. i. splits; ss. reflexivity.
-      - exploit Local.read_step_future; eauto. i. splits; ss. reflexivity.
+      - exploit Local.silent_step_future; eauto. i. splits; ss. refl.
+      - exploit Local.read_step_future; eauto. i. splits; ss. refl.
       - exploit Local.write_step_future; eauto.
       - exploit Local.read_step_future; eauto. i.
         exploit Local.write_step_future; eauto.
-      - exploit Local.fence_step_future; eauto. i. splits; ss. reflexivity.
+      - exploit Local.fence_step_future; eauto. i. splits; ss. refl.
     Qed.
 
     Lemma external_step_future e e1 e2
@@ -399,7 +386,7 @@ Module Thread.
       <<FUTURE: Memory.future e1.(memory) e2.(memory)>>.
     Proof.
       inv STEP. exploit Local.silent_step_future; eauto. i.
-      splits; ss. reflexivity.
+      splits; ss. refl.
     Qed.
 
     Lemma step_future e e1 e2
@@ -421,7 +408,7 @@ Module Thread.
       <<FUTURE: Memory.future e1.(memory) e2.(memory)>>.
     Proof.
       revert WF1. induction STEP.
-      - i. splits; ss. reflexivity.
+      - i. splits; ss. refl.
       - i.
         exploit step_future; eauto. i. des.
         exploit IHSTEP; eauto. i. des.
@@ -434,7 +421,6 @@ Module Thread.
         (DISJOINT1: Local.disjoint e1.(local) lc)
         (WF: Local.wf lc e1.(memory)):
       <<DISJOINT2: Local.disjoint e2.(local) lc>> /\
-      <<INTACT: Memory.intact lc.(Local.promises) e1.(memory) e2.(memory)>> /\
       <<WF: Local.wf lc e2.(memory)>>.
     Proof.
       inv STEP.
@@ -448,16 +434,13 @@ Module Thread.
         (DISJOINT1: Local.disjoint e1.(local) lc)
         (WF: Local.wf lc e1.(memory)):
       <<DISJOINT2: Local.disjoint e2.(local) lc>> /\
-      <<INTACT: Memory.intact lc.(Local.promises) e1.(memory) e2.(memory)>> /\
       <<WF: Local.wf lc e2.(memory)>>.
     Proof.
       inv STEP.
       - exploit Local.silent_step_future; eauto. i.
-        exploit Local.silent_step_disjoint; eauto. i.
-        splits; eauto. reflexivity.
+        exploit Local.silent_step_disjoint; eauto.
       - exploit Local.read_step_future; eauto. i.
-        exploit Local.read_step_disjoint; eauto. i.
-        splits; eauto. reflexivity.
+        exploit Local.read_step_disjoint; eauto.
       - exploit Local.write_step_future; eauto. i. des.
         exploit Local.write_step_disjoint; eauto.
       - exploit Local.read_step_future; eauto. i.
@@ -465,8 +448,7 @@ Module Thread.
         exploit Local.write_step_future; eauto. i. des.
         exploit Local.write_step_disjoint; eauto.
       - exploit Local.fence_step_future; eauto. i.
-        exploit Local.fence_step_disjoint; eauto. i.
-        splits; eauto. reflexivity.
+        exploit Local.fence_step_disjoint; eauto.
     Qed.
 
     Lemma external_step_disjoint e e1 e2 lc
@@ -475,12 +457,10 @@ Module Thread.
         (DISJOINT1: Local.disjoint e1.(local) lc)
         (WF: Local.wf lc e1.(memory)):
       <<DISJOINT2: Local.disjoint e2.(local) lc>> /\
-      <<INTACT: Memory.intact lc.(Local.promises) e1.(memory) e2.(memory)>> /\
       <<WF: Local.wf lc e2.(memory)>>.
     Proof.
       inv STEP. exploit Local.silent_step_future; eauto. i.
-      exploit Local.silent_step_disjoint; eauto. i.
-      splits; eauto. reflexivity.
+      exploit Local.silent_step_disjoint; eauto.
     Qed.
 
     Lemma step_disjoint e e1 e2 lc
@@ -489,7 +469,6 @@ Module Thread.
         (DISJOINT1: Local.disjoint e1.(local) lc)
         (WF: Local.wf lc e1.(memory)):
       <<DISJOINT2: Local.disjoint e2.(local) lc>> /\
-      <<INTACT: Memory.intact lc.(Local.promises) e1.(memory) e2.(memory)>> /\
       <<WF: Local.wf lc e2.(memory)>>.
     Proof.
       inv STEP.
@@ -504,15 +483,12 @@ Module Thread.
         (DISJOINT1: Local.disjoint e1.(local) lc)
         (WF: Local.wf lc e1.(memory)):
       <<DISJOINT2: Local.disjoint e2.(local) lc>> /\
-      <<INTACT: Memory.intact lc.(Local.promises) e1.(memory) e2.(memory)>> /\
       <<WF: Local.wf lc e2.(memory)>>.
     Proof.
-      revert WF1 DISJOINT1 WF. induction STEP; eauto; i.
-      { splits; eauto. reflexivity. }
+      revert WF1 DISJOINT1 WF. induction STEP; eauto. i.
       exploit step_future; eauto. i. des.
       exploit step_disjoint; eauto. i. des.
-      exploit IHSTEP; eauto. i. des.
-      splits; eauto. etrans; eauto.
+      exploit IHSTEP; eauto.
     Qed.
   End Thread.
 End Thread.
