src/opt/MemInv.v
@@ -27,7 +27,7 @@ Inductive sim_memory (mem_src mem_tgt:Memory.t): Prop :=
 .
 
 Program Instance sim_memory_PreOrder: PreOrder sim_memory.
-Next Obligation. ii. econs. reflexivity. Qed.
+Next Obligation. ii. econs. refl. Qed.
 Next Obligation. ii. inv H. inv H0. econs. etrans; eauto. Qed.
 
 Lemma sim_memory_get
@@ -41,12 +41,177 @@ Proof.
 Qed.
 
 Module MemInv.
-  Definition t := Promises.t.
+  Definition t := Loc.t -> DOSet.t.
 
-  Inductive sem (inv:t) (promises_src promises_tgt:Promises.t): Prop :=
+  Definition mem loc ts (promises:t) := DOSet.mem ts (promises loc).
+
+  Lemma ext lhs rhs
+        (EXT: forall loc ts, mem loc ts lhs = mem loc ts rhs):
+    lhs = rhs.
+  Proof.
+    extensionality loc.
+    apply DOSet.eq_leibniz. ii.
+    specialize (EXT loc a). unfold mem in *. econs; i.
+    - apply DOSet.mem_spec. erewrite <- EXT.
+      apply DOSet.mem_spec. auto.
+    - apply DOSet.mem_spec. erewrite EXT.
+      apply DOSet.mem_spec. auto.
+  Qed.
+
+  Definition bot: t := fun _ => DOSet.empty.
+
+  Lemma bot_spec loc ts: mem loc ts bot = false.
+  Proof.
+    unfold mem, bot. apply DOSet.Facts.empty_b.
+  Qed.
+
+  Definition le (lhs rhs:t): Prop :=
+    forall loc ts, mem loc ts lhs -> mem loc ts rhs.
+
+  Definition join (lhs rhs:t): t :=
+    fun loc => DOSet.union (lhs loc) (rhs loc).
+
+  Lemma join_comm lhs rhs: join lhs rhs = join rhs lhs.
+  Proof.
+    unfold join. extensionality loc.
+    apply DOSet.eq_leibniz. ii.
+    rewrite ? DOSet.union_spec. econs; i; des; auto.
+  Qed.
+
+  Lemma join_assoc a b c: join (join a b) c = join a (join b c).
+  Proof.
+    unfold join. extensionality loc.
+    apply DOSet.eq_leibniz. ii.
+    rewrite ? DOSet.union_spec. econs; i; des; auto.
+  Qed.
+
+  Lemma join_l lhs rhs: le lhs (join lhs rhs).
+  Proof.
+    unfold join. ii. unfold mem in *.
+    rewrite DOSet.Facts.union_b, H. auto.
+  Qed.
+
+  Lemma join_r lhs rhs: le rhs (join lhs rhs).
+  Proof. rewrite join_comm. apply join_l. Qed.
+
+  Lemma join_spec lhs rhs o
+        (LHS: le lhs o)
+        (RHS: le rhs o):
+    le (join lhs rhs) o.
+  Proof.
+    unfold join. ii.
+    unfold mem in *. rewrite DOSet.Facts.union_b in *.
+    apply Bool.orb_true_iff in H. des; eauto.
+  Qed.
+
+  Definition set (loc:Loc.t) (ts:Time.t) (promises:t) :=
+    LocFun.add loc (DOSet.add ts (promises loc)) promises.
+
+  Lemma set_o loc1 ts1 loc2 ts2 promises:
+    mem loc1 ts1 (set loc2 ts2 promises) =
+    if andb (if Loc.eq_dec loc1 loc2 then true else false) (if Time.eq_dec ts1 ts2 then true else false)
+    then true
+    else mem loc1 ts1 promises.
+  Proof.
+    unfold mem, set, LocFun.add, LocFun.find.
+    destruct (Loc.eq_dec loc1 loc2); subst; ss.
+    destruct (Time.eq_dec ts1 ts2); subst; ss.
+    - rewrite DOSet.Facts.add_b.
+      unfold DOSet.Facts.eqb. destruct (Time.eq_dec ts2 ts2); auto.
+    - rewrite DOSet.Facts.add_b.
+      unfold DOSet.Facts.eqb. destruct (Time.eq_dec ts2 ts1); ss.
+      congr.
+  Qed.
+
+  Lemma set_eq loc ts promises:
+    mem loc ts (set loc ts promises) = true.
+  Proof.
+    rewrite set_o.
+    destruct (Loc.eq_dec loc loc); [|congr].
+    destruct (Time.eq_dec ts ts); [|congr].
+    auto.
+  Qed.
+
+  Lemma set_inv loc1 ts1 loc2 ts2 promises
+        (MEM: mem loc1 ts1 (set loc2 ts2 promises)):
+    (loc1 = loc2 /\ ts1 = ts2) \/ mem loc1 ts1 promises.
+  Proof.
+    rewrite set_o in MEM.
+    destruct (Loc.eq_dec loc1 loc2); ss; auto.
+    destruct (Time.eq_dec ts1 ts2); ss; auto.
+  Qed.
+
+  Definition unset (loc:Loc.t) (ts:Time.t) (promises:t) :=
+    LocFun.add loc (DOSet.remove ts (promises loc)) promises.
+
+  Lemma unset_o loc1 ts1 loc2 ts2 promises:
+    mem loc1 ts1 (unset loc2 ts2 promises) =
+    if andb (if Loc.eq_dec loc1 loc2 then true else false) (if Time.eq_dec ts1 ts2 then true else false)
+    then false
+    else mem loc1 ts1 promises.
+  Proof.
+    unfold mem, unset, LocFun.add, LocFun.find.
+    destruct (Loc.eq_dec loc1 loc2); subst; ss.
+    destruct (Time.eq_dec ts1 ts2); subst; ss.
+    - rewrite DOSet.Facts.remove_b.
+      unfold DOSet.Facts.eqb. destruct (Time.eq_dec ts2 ts2); [|congr].
+      apply Bool.andb_false_iff. auto.
+    - rewrite DOSet.Facts.remove_b.
+      unfold DOSet.Facts.eqb. destruct (Time.eq_dec ts2 ts1); ss; [congr|].
+      apply Bool.andb_true_r.
+  Qed.
+
+  Lemma unset_eq loc ts promises:
+    mem loc ts (unset loc ts promises) = false.
+  Proof.
+    rewrite unset_o.
+    destruct (Loc.eq_dec loc loc); [|congr].
+    destruct (Time.eq_dec ts ts); [|congr].
+    auto.
+  Qed.
+
+  Lemma unset_inv loc1 ts1 loc2 ts2 promises
+        (MEM: mem loc1 ts1 (unset loc2 ts2 promises)):
+    ~ (loc1 = loc2 /\ ts1 = ts2) /\ mem loc1 ts1 promises.
+  Proof.
+    rewrite unset_o in MEM.
+    destruct (Loc.eq_dec loc1 loc2), (Time.eq_dec ts1 ts2); ss; splits; auto.
+    - contradict n. des. auto.
+    - contradict n. des. auto.
+    - contradict n. des. auto.
+  Qed.
+
+  Lemma unset_set loc to inv
+        (MEM: mem loc to inv = false):
+    unset loc to (set loc to inv) = inv.
+  Proof.
+    apply ext. i.
+    rewrite unset_o, set_o.
+    destruct (Loc.eq_dec loc0 loc), (Time.eq_dec ts to); ss; splits; auto.
+    subst. auto.
+  Qed.
+
+  Inductive disjoint (lhs rhs:t): Prop :=
+  | disjoint_intro
+      (DISJOINT: forall loc ts
+                   (LHS: mem loc ts lhs)
+                   (RHS: mem loc ts rhs),
+          False).
+
+  Global Program Instance disjoint_Symmetric: Symmetric disjoint.
+  Next Obligation.
+    econs. ii. eapply H; eauto.
+  Qed.
+
+  Inductive sem (inv:t) (promises_src promises_tgt:Memory.t): Prop :=
   | sem_intro
-      (DISJOINT: Promises.disjoint promises_tgt inv)
-      (JOIN: promises_src = Promises.join inv promises_tgt)
+      (LE: Memory.le promises_tgt promises_src)
+      (GET: forall loc ts (MEM: mem loc ts inv),
+          Memory.get loc ts promises_src <> None /\ Memory.get loc ts promises_tgt = None)
+      (MEM: forall loc ts
+              (SRC: Memory.get loc ts promises_src <> None)
+              (TGT: Memory.get loc ts promises_tgt = None),
+          mem loc ts inv)
   .
 
   Lemma promise
@@ -57,12 +222,14 @@ Module MemInv.
         (PROMISES_TGT: Memory.promise promises1_tgt mem1_tgt loc from to msg promises2_tgt mem2_tgt)
         (INV1: sem inv promises1_src promises1_tgt)
         (SIM1: sim_memory mem1_src mem1_tgt)
-        (WF1_PROMISES_SRC: Memory.closed_promises promises1_src mem1_src)
-        (WF1_PROMISES_TGT: Memory.closed_promises promises1_tgt mem1_tgt):
+        (LE_SRC1: Memory.le promises1_src mem1_src)
+        (LE_TGT1: Memory.le promises1_tgt mem1_tgt)
+        (CLOSED_SRC1: Memory.closed mem1_src)
+        (CLOSED_TGT1: Memory.closed mem1_tgt):
     exists promises2_src mem2_src,
       <<PROMISES_SRC: Memory.promise promises1_src mem1_src loc from to msg promises2_src mem2_src>> /\
       <<INV2: sem inv promises2_src promises2_tgt>> /\
-      <<WF1_PROMISES_SRC: Memory.closed_promises promises2_src mem2_src>> /\
+      <<LE_SRC1: Memory.le promises2_src mem2_src>> /\
       <<SIM2: sim_memory mem2_src mem2_tgt>>.
   Proof.
   Admitted.
@@ -70,37 +237,25 @@ Module MemInv.
   Lemma fulfill_tgt
         inv
         promises1_src
-        promises1_tgt mem1_tgt promises2_tgt
+        promises1_tgt promises2_tgt
         loc from to msg
-        (FULFILL_TGT: Memory.fulfill promises1_tgt mem1_tgt loc from to msg promises2_tgt)
-        (INV1: sem inv promises1_src promises1_tgt):
-    <<DISJOINT: ~ Promises.mem loc to inv>> /\
-    <<INV2: sem (Promises.set loc to inv) promises1_src promises2_tgt>>.
+        (FULFILL_TGT: Memory.fulfill promises1_tgt loc from to msg promises2_tgt)
+        (INV: sem inv promises1_src promises1_tgt):
+    sem (set loc to inv) promises1_src promises2_tgt.
   Proof.
-    inv INV1. inv FULFILL_TGT.
-    splits.
-    - ii. eapply DISJOINT; eauto.
-    - econs.
-      + admit.
-      + admit.
   Admitted.
 
   Lemma fulfill_src
-        inv1 inv2
-        promises1_src mem1_src
+        inv
+        promises1_src
         promises1_tgt
         loc from to msg
-        (FULFILL_INV: Memory.fulfill inv1 mem1_src loc from to msg inv2)
-        (INV1: sem inv1 promises1_src promises1_tgt):
+        (TGT: Memory.get loc to promises1_tgt = None)
+        (INV1: sem inv promises1_src promises1_tgt):
     exists promises2_src,
-      <<FULFILL_SRC: Memory.fulfill promises1_src mem1_src loc from to msg promises2_src>> /\
-      <<INV2: sem inv2 promises2_src promises1_tgt>>.
+      <<FULFILL_SRC: Memory.fulfill promises1_src loc from to msg promises2_src>> /\
+      <<INV2: sem (unset loc to inv) promises2_src promises1_tgt>>.
   Proof.
-    inv INV1. eexists. splits.
-    - inv FULFILL_INV. econs; eauto. admit.
-    - econs.
-      + admit.
-      + admit.
   Admitted.
 
   Lemma fulfill
@@ -108,33 +263,24 @@ Module MemInv.
         loc from to msg
         promises1_src mem1_src
         promises1_tgt mem1_tgt promises2_tgt
-        (FULFILL_TGT: Memory.fulfill promises1_tgt mem1_tgt loc from to msg promises2_tgt)
+        (FULFILL_TGT: Memory.fulfill promises1_tgt loc from to msg promises2_tgt)
         (INV1: sem inv promises1_src promises1_tgt)
         (SIM1: sim_memory mem1_src mem1_tgt)
-        (WF1_PROMISES_SRC: Memory.closed_promises promises1_src mem1_src)
-        (WF1_PROMISES_TGT: Memory.closed_promises promises1_tgt mem1_tgt)
-        (WF1_SRC: Memory.closed mem1_src):
+        (LE_SRC1: Memory.le promises1_src mem1_src)
+        (LE_TGT1: Memory.le promises1_tgt mem1_tgt)
+        (CLOSED_SRC1: Memory.closed mem1_src)
+        (CLOSED_TGT1: Memory.closed mem1_tgt):
     exists promises2_src,
-      <<FULFILL_SRC: Memory.fulfill promises1_src mem1_src loc from to msg promises2_src>> /\
-      <<INV2: sem inv promises2_src promises2_tgt>> /\
-      <<WF1_PROMISES_SRC: Memory.closed_promises promises2_src mem1_src>>.
+      <<FULFILL_SRC: Memory.fulfill promises1_src loc from to msg promises2_src>> /\
+      <<INV2: sem inv promises2_src promises2_tgt>>.
   Proof.
-    exploit fulfill_tgt; eauto. i. des.
-    exploit fulfill_src; try apply INV2; eauto.
-    { econs.
-      - inv FULFILL_TGT. eauto.
-      - rewrite Promises.set_o.
-        destruct (Loc.eq_dec loc loc); [|congruence].
-        destruct (Time.eq_dec to to); [|congruence].
-        auto.
-    }
+    exploit fulfill_tgt; eauto. i.
+    exploit fulfill_src; eauto.
+    { inv x0. eapply GET; eauto. apply set_eq. }
     i. des.
-    exploit Memory.fulfill_mon; eauto; i.
-    { apply Memory.splits_future. apply SIM1. }
-    { admit. }
     eexists. splits; eauto.
-    - admit.
-    - eapply Memory.fulfill_future; eauto.
+    rewrite unset_set in INV2; auto.
+    admit.
   Admitted.
 
   Lemma future
@@ -144,38 +290,38 @@ Module MemInv.
         (FUTURE_SRC: Memory.future mem1_src mem2_src)
         (INV1: sem inv promises_src promises_tgt)
         (SIM1: sim_memory mem1_src mem1_tgt)
-        (WF1_PROMISES_SRC: Memory.closed_promises promises_src mem1_src)
-        (WF1_PROMISES_TGT: Memory.closed_promises promises_tgt mem1_tgt)
-        (WF2_PROMISES_SRC: Memory.closed_promises promises_src mem2_src):
+        (LE_SRC1: Memory.le promises_src mem1_src)
+        (LE_TGT1: Memory.le promises_tgt mem1_tgt)
+        (LE_SRC2: Memory.le promises_src mem2_src):
       <<FUTURE_TGT: Memory.future mem1_tgt mem2_src>> /\
-      <<WF2_PROMISES_TGT: Memory.closed_promises promises_tgt mem2_src>>.
+      <<WF2_PROMISES_TGT: Memory.le promises_tgt mem2_src>>.
   Proof.
-    revert INV1 SIM1 WF1_PROMISES_SRC WF1_PROMISES_TGT WF2_PROMISES_SRC.
-    revert inv mem1_tgt promises_src promises_tgt.
-    induction FUTURE_SRC; i.
-    - splits.
-      + apply Memory.splits_future. apply SIM1.
-      + admit.
-    - inv H.
-      + admit.
-      + eapply IHFUTURE_SRC; eauto.
-        * admit.
-        * admit.
-  Admitted.
+    splits.
+    - etrans; eauto. apply Memory.splits_future. apply SIM1.
+    - etrans; [apply INV1|]. eauto.
+  Qed.
 
-  Lemma sem_bot promise:
-    sem Promises.bot promise promise.
+  Lemma sem_bot promises:
+    sem bot promises promises.
   Proof.
     econs.
-    - admit.
-    - admit.
-  Admitted.
+    - refl.
+    - i. rewrite bot_spec in MEM. done.
+    - congr.
+  Qed.
 
   Lemma sem_bot_inv
-        promises_src promises_tgt
-        (SEM: sem Promises.bot promises_src promises_tgt):
-    promises_src = promises_tgt.
+        promises
+        (SEM: sem bot promises Memory.bot):
+    promises = Memory.bot.
   Proof.
-    inv SEM. admit.
-  Admitted.
+    extensionality loc. apply Cell.ext. s.
+    apply DOMap.eq_leibniz. ii.
+    unfold Cell.Raw.bot. rewrite DOMap.gempty.
+    destruct (DOMap.find y (Cell.raw (promises loc))) eqn:X; auto.
+    inv SEM.  exploit MEM.
+    - unfold Memory.get, Cell.get. rewrite X. congr.
+    - apply Memory.bot_get.
+    - i. rewrite bot_spec in x. congr.
+  Qed.
 End MemInv.
